platform/tests/BabyThread.v
@@ -4,16 +4,21 @@ Require Import Thread.
 Definition handlerS := SPECthd reserving 14
   PREonly[_] Emp.
 
-Definition mainS := SPEC reserving 15
+Definition mainS := SPEC reserving 23
   PREonly[_] mallocHeap 0.
 
-Definition m := bimport [[ "scheduler"!"init" @ [initS], "scheduler"!"exit" @ [exitS] ]]
+Definition m := bimport [[ "scheduler"!"init" @ [initS], "scheduler"!"exit" @ [exitS],
+                           "scheduler"!"spawn" @ [spawnS] ]]
   bmodule "test" {{
     tfunctionNoRet "handler"() [handlerS]
-      Exit
+      Diverge
+      (*Exit*)
     end with bfunctionNoRet "main"("sc") [mainS]
       "sc" <-- Call "scheduler"!"init"()
       [PREonly[_, R] sched R * mallocHeap 0];;
+
+      Spawn("sc", "test"!"handler", 16)
+      [PREonly[V] sched (V "sc") * mallocHeap 0];;
 
       Go "sc"
     end
@@ -24,13 +29,82 @@ Theorem ok : moduleOk m.
 
   sep_auto.
   sep_auto.
-  sep_auto.
-  sep_auto.
+  (*sep_auto.
+  sep_auto.*)
 
   sep_auto.
   sep_auto.
   sep_auto.
   sep_auto.
+  sep_auto.
+  sep_auto.
+  sep_auto.
+
+  post.
+  evaluate auto_ext.
+  descend.
+
+  Ltac toFront_conc which :=
+    let rec toFront' P k :=
+      match P with
+        | SEP.ST.star ?Q ?R =>
+          toFront' Q ltac:(fun it P' => k it (SEP.ST.star P' R))
+          || toFront' R ltac:(fun it P' => k it (SEP.ST.star P' Q))
+        | (?Q * ?R)%Sep =>
+          toFront' Q ltac:(fun it P' => k it (SEP.ST.star P' R))
+          || toFront' R ltac:(fun it P' => k it (SEP.ST.star P' Q))
+        | _ => which P; k P (@SEP.ST.emp W (settings * state) nil)
+      end in
+      match goal with
+        | [ |- interp ?specs (![ ?P ] ?st) ] => toFront' P ltac:(fun it P' =>
+          let H := fresh "H" in assert (H : interp specs (![ SEP.ST.star it P' ] st)); [ |
+            generalize dependent H;
+              repeat match goal with
+                       | [ H : interp _ _ |- _ ] => clear H
+                     end; intro; eapply Imply_sound; [ eapply sepFormula_himp_imply | ];
+              [ | reflexivity | eassumption ]; solve [ step auto_ext ] ])
+      end.
+
+  toFront_conc ltac:(fun P => match P with
+                                | starting _ _ _ => idtac
+                              end).
+  apply starting_intro.
+  descend.
+  Focus 2.
+  sep_auto.
+  discriminate.
+  eauto.
+  unfold threadInvariantCont.
+  descend.
+  apply andL; apply injL; intro.
+  apply andL; apply injL; intro.
+  apply andL; apply cptrL; intro.
+  apply andL; apply injL; intro.
+  eapply existsXR; unfold Subst; simpl.
+  eapply existsR.
+  apply andR.
+  eapply existsXR; unfold Subst; simpl.
+  descend.
+  apply andL; apply implyR.
+  instantiate (1 := fun p => Emp%Sep (fst p) (snd p)).
+  instantiate (1 := fun p => sched_ (fst p) (snd p)).
+  instantiate (1 := vs).
+  clear.
+  step auto_ext.
+  eapply existsR.
+  apply andR.
+  apply injR; eauto.
+  apply (f_equal (fun f => f (labl "scheduler" "exit"))) in H11.
+  etransitivity; eassumption.
+  eapply existsXR; unfold Subst; simpl.
+  apply andR.
+  apply cptrR; eauto.
+  apply andL; apply swap; apply implyR.
+  rewrite H13; rewrite <- H11; rewrite sepFormula_eq; apply Imply_refl.
+  step auto_ext.
+  descend; step auto_ext.
+  descend; step auto_ext.
+  
   sep_auto.
   sep_auto.
   sep_auto.
